# $\gamma^5$
Proof of $\gamma^5$ form in Dirac basis:

$$
\begin{aligned}
\gamma^5&\equiv i\gamma^0\gamma^1\gamma^2\gamma^3
 = i\gamma^0\gamma^1\gamma^2(\gamma^0\gamma^0)\gamma^3
 = i(\gamma^0\gamma^1)(\gamma^2\gamma^0)(\gamma^0\gamma^3)\\[8pt]
&= i\left(\begin{array}{ll}
0 & \sigma^1\\
\sigma^1 & 0
\end{array}
\right)
\left(\begin{array}{cc}
0 & -\sigma^2\\
-\sigma^2 & 0
\end{array}
\right)
\left(\begin{array}{ll}
0 & \sigma^3\\
\sigma^3 & 0
\end{array}
\right)\\[8pt]
&=
\left(\begin{array}{cc}
0 & -i\sigma^1\sigma^2\sigma^3\\
-i\sigma^1\sigma^2\sigma^3 & 0
\end{array}
\right)\\[8pt]
&=
\left(\begin{array}{cc}
0 & 1\\
1 & 0
\end{array}
\right)
\end{aligned}
$$